finished correctness of compiler, termination left

theories/TM/Compound/Compare.v
@@ -1,11 +1,11 @@
+Require Import FunInd.
+
 From Undecidability Require Import TM.Util.Prelim.
 From Undecidability Require Import TM.Basic.Basic.
 From Undecidability Require Import TM.Combinators.Combinators.
-From Undecidability Require Import TM.Compound.TMTac.
-From Undecidability Require Import TM.Compound.Multi.
+From Undecidability.TM.Compound Require Import TMTac Multi MoveToSymbol.
 
-From Coq Require Import FunInd.
-From Coq Require Import Recdef.
+Require Recdef.
 
 
 (** * Compare two tapes (from left to right) until a symbol is reached *)
@@ -14,6 +14,7 @@ From Coq Require Import Recdef.
 
 
 Section Compare.
+  Import Recdef.
 
   Variable sig : finType.
   Variable stop : sig -> bool. (* stop symbol(s) *)
@@ -151,3 +152,309 @@ Section Compare.
     
 
 End Compare.
+
+
+Section CompareLists.
+
+  Variable X : eqType.
+  
+  Definition list_comperasion (xs ys : list X) : Prop :=
+    xs = ys \/
+    (exists a b l1 l2 l3, a <> b /\ xs = l1 ++ a :: l2 /\ ys = l1 ++ b :: l3) \/
+    (exists a l1 l2, xs = l1 ++ a :: l2 /\ ys = l1) \/
+    (exists a l1 l2, xs = l1 /\ ys = l1 ++ a :: l2).
+
+  Definition list_comperasion_cons xs ys x :
+    list_comperasion xs ys ->
+    list_comperasion (x :: xs) (x :: ys).
+  Proof.
+    destruct 1 as [ <- | [ (a&b&l1&l2&l3&H1&H2&H3) | [ (a&l1&l2&H1&H2) | (a&l1&l2&H1&H2) ]]].
+    - left. reflexivity.
+    - subst. right; left. exists a, b, (x::l1), l2, l3. auto.
+    - subst. right. right. left. do 3 eexists. split. 2: reflexivity. cbn. eauto.
+    - subst. right. right. right. do 3 eexists. split. 1: reflexivity. cbn. eauto.
+  Qed.
+
+  Lemma compare_lists (xs ys : list X) :
+    list_comperasion xs ys.
+  Proof.
+    revert ys. induction xs as [ | x xs IH]; intros; cbn in *.
+    - destruct ys as [ | y ys].
+      + left. reflexivity.
+      + right. right. right. do 3 eexists. split. reflexivity. cbn. reflexivity.
+    - destruct ys as [ | y ys].
+      + hnf. right. right. left. do 3 eexists. split. 2: reflexivity. cbn. reflexivity.
+      + decide (x = y) as [ <- | HDec].
+        * now apply list_comperasion_cons.
+        * hnf. right. left. exists x, y, nil. cbn. do 2 eexists. eauto.
+  Qed.
+
+End CompareLists.
+
+
+Local Arguments plus : simpl never.
+Local Arguments mult : simpl never.
+
+Section Compare_fun_lemmas.
+
+  Variable (X : finType) (stop : X -> bool).
+
+
+  Lemma Compare_correct_eq (str : list X) (s1 s2 : X) rs1 rs2 t :
+    (forall x, In x str -> stop x = false) ->
+    stop s1 = true ->
+    stop s2 = true ->
+    tape_local (fst t) = str ++ s1 :: rs1 ->
+    tape_local (snd t) = str ++ s2 :: rs2 ->
+    Compare_fun stop t =
+    (true, (midtape (rev str ++ left (fst t)) s1 rs1, midtape (rev str ++ left (snd t)) s2 rs2)).
+  Proof.
+    revert str s1 s2 rs1 rs2. functional induction (Compare_fun stop t); intros str s1 s2 rs1 rs2 HStr HS1 HS2 HL1 HL2; destruct t as [t1 t2]; cbn in *;
+                                try rewrite HS1 in *; try rewrite HS2 in *; cbn in *; auto.
+    - destruct str as [ | s str']; cbn in *.
+      + apply midtape_tape_local_cons in HL1 as ->. apply midtape_tape_local_cons in HL2 as ->. cbn. reflexivity.
+      + apply midtape_tape_local_cons in HL1. apply midtape_tape_local_cons in HL2.
+        rewrite HL1 in *. cbn in *. inv e. rewrite HL2 in *. cbn in *. inv e0.
+        specialize (HStr c2 ltac:(auto)). rewrite HStr in e1. cbn in *. congruence.
+    - (* absurd case *) exfalso. destruct str as [ | s str']; cbn in *.
+      + apply midtape_tape_local_cons in HL1. apply midtape_tape_local_cons in HL2. rewrite HL1, HL2 in *. cbn in *. inv e; inv e0. rewrite HS1, HS2 in e1. cbn in *. congruence.
+      + apply midtape_tape_local_cons in HL1. apply midtape_tape_local_cons in HL2. rewrite HL1, HL2 in *. cbn in *. inv e; inv e0.
+        specialize (HStr c2 ltac:(auto)). rewrite HStr in *. cbn in *. congruence.
+    - (* Induction case *) destruct str as [ | s str']; cbn in *.
+      + exfalso. apply midtape_tape_local_cons in HL1. apply midtape_tape_local_cons in HL2. rewrite HL1, HL2 in *. cbn in *. inv e; inv e0. rewrite HS1 in e1. cbn in *. congruence.
+      + apply midtape_tape_local_cons in HL1. apply midtape_tape_local_cons in HL2. rewrite HL1, HL2 in *. cbn in *. inv e; inv e0.
+        apply orb_false_iff in e2 as (e2&_).
+        simpl_tape in IHp. specialize IHp with (4 := eq_refl) (5 := eq_refl) (2 := HS1) (3 := HS2). spec_assert IHp by auto.
+        simpl_list; cbn; auto.
+    - (* absurd case *) exfalso. destruct str as [ | s str']; cbn in *.
+      + apply midtape_tape_local_cons in HL1. apply midtape_tape_local_cons in HL2. rewrite HL1, HL2 in *. cbn in *. inv e; inv e0. rewrite HS1, HS2 in e1. cbn in *. congruence.
+      + apply midtape_tape_local_cons in HL1. apply midtape_tape_local_cons in HL2. rewrite HL1, HL2 in *. cbn in *. inv e; inv e0.
+        specialize (HStr c2 ltac:(auto)). rewrite HStr in *. cbn in *. congruence.
+    - (* absurd case *) exfalso. destruct str as [ | s str']; cbn in *.
+      + apply midtape_tape_local_cons in HL1. apply midtape_tape_local_cons in HL2. rewrite HL1, HL2 in *. cbn in *. auto.
+      + apply midtape_tape_local_cons in HL1. apply midtape_tape_local_cons in HL2. rewrite HL1, HL2 in *. cbn in *. auto.
+  Qed.
+
+  Lemma Compare_correct_eq_midtape (str : list X) (s1 s2 : X) ls1 rs1 ls2 m rs2 :
+    (forall x, In x str -> stop x = false) ->
+    stop m = false ->
+    stop s1 = true ->
+    stop s2 = true ->
+    Compare_fun stop (midtape ls1 m (str ++ s1 :: rs1), midtape ls2 m (str ++ s2 :: rs2)) =
+    (true, (midtape (rev str ++ m :: ls1) s1 rs1, midtape (rev str ++ m :: ls2) s2 rs2)).
+  Proof.
+    intros HStr Hm HS1 HS2.
+    rewrite Compare_fun_equation; cbn. erewrite Compare_correct_eq with (str := str) (rs1 := rs1) (rs2 := rs2) (s1 := s1) (s2 := s2); eauto.
+    all: cbn; simpl_tape; auto.
+    rewrite Hm. cbn. decide (m=m); [ | tauto]. now simpl_tape.
+  Qed.
+
+
+  Lemma Compare_correct_neq (str1 str2 str3 : list X) (x1 x2 : X) t :
+    (forall x, In x str1 -> stop x = false) ->
+    stop x1 = false ->
+    stop x2 = false ->
+    x1 <> x2 ->
+    tape_local (fst t) = str1 ++ x1 :: str2 ->
+    tape_local (snd t) = str1 ++ x2 :: str3 ->
+    Compare_fun stop t =
+    (false, (midtape (rev str1 ++ left (fst t)) x1 str2, midtape (rev str1 ++ left (snd t)) x2 str3)).
+  Proof.
+    revert str1 str2 str3 x1 x2. functional induction (Compare_fun stop t); intros str1 str2 str3 x1 x2; intros Hstr1 Hx1 Hx2 Hx12 HT1 HT2; destruct t as [t1 t2]; cbn in *.
+    - exfalso. destruct str1 as [ | s str1]; cbn in *.
+      + apply midtape_tape_local_cons in HT1. apply midtape_tape_local_cons in HT2. rewrite HT1, HT2 in *. cbn in *. inv e; inv e0. rewrite Hx1 in e1. cbn in *. congruence.
+      + apply midtape_tape_local_cons in HT1. apply midtape_tape_local_cons in HT2. rewrite HT1, HT2 in *. cbn in *. specialize (Hstr1 s ltac:(eauto)). inv e; inv e0.
+        rewrite Hstr1 in e1. cbn in *. congruence.
+    - exfalso. destruct str1 as [ | s str1]; cbn in *.
+      + apply midtape_tape_local_cons in HT1. apply midtape_tape_local_cons in HT2. rewrite HT1, HT2 in *. cbn in *. inv e; inv e0. rewrite Hx1 in e2. cbn in *. congruence.
+      + apply midtape_tape_local_cons in HT1. apply midtape_tape_local_cons in HT2. rewrite HT1, HT2 in *. cbn in *. specialize (Hstr1 s ltac:(eauto)).
+        inv e; inv e0. rewrite Hstr1 in e2. cbn in *. congruence.
+    - (* inductive case *) destruct str1 as [ | s str1]; cbn in *.
+      + apply midtape_tape_local_cons in HT1. apply midtape_tape_local_cons in HT2. rewrite HT1, HT2 in *. cbn in *. inv e; inv e0. tauto.
+      + apply midtape_tape_local_cons in HT1. apply midtape_tape_local_cons in HT2. rewrite HT1, HT2 in *. cbn in *. inv e; inv e0.
+        simpl_tape in IHp. specialize IHp with (5 := eq_refl) (6 := eq_refl) (2 := Hx1) (3 := Hx2) (4 := Hx12). spec_assert IHp by auto.
+        simpl_list; cbn; auto.
+    - destruct str1 as [ | s str1]; cbn in *.
+      + apply midtape_tape_local_cons in HT1. apply midtape_tape_local_cons in HT2. rewrite HT1, HT2 in *. cbn in *. inv e; inv e0. rewrite Hx1 in e2. cbn in *. congruence.
+      + apply midtape_tape_local_cons in HT1. apply midtape_tape_local_cons in HT2. rewrite HT1, HT2 in *. cbn in *. inv e; inv e0. now contradiction _x.
+    - exfalso. destruct str1 as [ | s str1]; cbn in *.
+      + apply midtape_tape_local_cons in HT1. apply midtape_tape_local_cons in HT2. rewrite HT1, HT2 in *. cbn in *. auto.
+      + apply midtape_tape_local_cons in HT1. apply midtape_tape_local_cons in HT2. rewrite HT1, HT2 in *. cbn in *. auto.
+  Qed.
+
+  Lemma Compare_correct_neq_midtape (str1 str2 str3 : list X) (m x1 x2 : X) ls1 ls2 :
+    (forall x, In x str1 -> stop x = false) ->
+    stop x1 = false ->
+    stop x2 = false ->
+    stop m = false ->
+    x1 <> x2 ->
+    Compare_fun stop (midtape ls1 m (str1 ++ x1 :: str2), midtape ls2 m (str1 ++ x2 :: str3)) =
+    (false, (midtape (rev str1 ++ m :: ls1) x1 str2, midtape (rev str1 ++ m :: ls2) x2 str3)).
+  Proof.
+    intros Hstr1 Hx1 Hx2 Hm Hx12.
+    rewrite Compare_fun_equation; cbn. rewrite Compare_correct_neq with (str1 := str1) (str2 := str2) (str3 := str3) (x1 := x1) (x2 := x2).
+    all: cbn; simpl_tape; auto.
+    rewrite Hm. cbn. decide (m=m); [ | tauto]. now simpl_tape.
+  Qed.
+
+
+  Definition swap (A B : Type) : A*B->B*A := ltac:(intros [b a]; now constructor).
+
+  Lemma Compare_correct_swap t :
+    Compare_fun stop (swap t) = (fst (Compare_fun stop t), swap (snd (Compare_fun stop t))).
+  Proof.
+    functional induction (Compare_fun stop t); destruct t as [t1 t2]; cbn in *.
+    - rewrite Compare_fun_equation. cbn. rewrite e, e0.
+      rewrite andb_comm in e1. now rewrite e1.
+    - rewrite Compare_fun_equation. cbn. rewrite e, e0.
+      rewrite andb_comm in e1. rewrite orb_comm in e2. now rewrite e1, e2.
+    - rewrite Compare_fun_equation. cbn. rewrite e, e0.
+      rewrite e1, e2. decide (c1=c1) as [ ? | H]; [ | now contradiction H]. auto.
+    - rewrite Compare_fun_equation. cbn. rewrite e, e0.
+      rewrite andb_comm in e1. rewrite orb_comm in e2. rewrite e1, e2.
+      decide (c2=c1) as [ <- | H]; [ now contradiction _x | ]. auto.
+    - rewrite Compare_fun_equation. cbn.
+      destruct (current t1); auto; destruct (current t2); auto.
+  Qed.
+
+
+  Lemma Compare_correct_short (str1 str2 rs1 rs2 : list X) (x : X) (s1 s2 : X) t :
+    (forall x, In x str1 -> stop x = false) ->
+    stop x = false ->
+    stop s1 = true ->
+    stop s2 = true ->
+    tape_local (fst t) = str1 ++ x :: str2 ++ s1 :: rs1 ->
+    tape_local (snd t) = str1 ++ s2 :: rs2 ->
+    Compare_fun stop t =
+    (false, (midtape (rev str1 ++ left (fst t)) x (str2 ++ s1 :: rs1),
+             midtape (rev str1 ++ left (snd t)) s2 rs2)).
+  Proof.
+    revert str1 str2 rs1 rs2 x s1 s2. functional induction (Compare_fun stop t); intros str1 str2 rs1 rs2 x s1 s2; intros Hstr1 Hx Hs1 Hs2 HT1 HT2; destruct t as [t1 t2]; cbn in *.
+    - exfalso. destruct str1 as [ | s str1]; cbn in *.
+      + apply midtape_tape_local_cons in HT1. apply midtape_tape_local_cons in HT2. rewrite HT1, HT2 in *. cbn in *. inv e; inv e0. rewrite Hx in e1. cbn in e1. congruence.
+      + apply midtape_tape_local_cons in HT1. apply midtape_tape_local_cons in HT2. rewrite HT1, HT2 in *. cbn in *. inv e; inv e0.
+        specialize (Hstr1 c2 ltac:(auto)). rewrite Hstr1 in e1. cbn in e1. congruence.
+    - destruct str1 as [ | s str1]; cbn in *.
+      + apply midtape_tape_local_cons in HT1. apply midtape_tape_local_cons in HT2. rewrite HT1, HT2 in *. cbn in *. auto.
+      + apply midtape_tape_local_cons in HT1. apply midtape_tape_local_cons in HT2. rewrite HT1, HT2 in *. cbn in *. inv e; inv e0.
+        specialize (Hstr1 c2 ltac:(auto)). rewrite Hstr1 in e2. cbn in e2. congruence.
+    - (* induction case *) destruct str1 as [ | s str1]; cbn in *.
+      + exfalso. apply midtape_tape_local_cons in HT1. apply midtape_tape_local_cons in HT2. rewrite HT1, HT2 in *. cbn in *. inv e; inv e0.
+        rewrite Hs2 in e1. cbn in e1. congruence.
+      + apply midtape_tape_local_cons in HT1. apply midtape_tape_local_cons in HT2. rewrite HT1, HT2 in *. cbn in *. inv e; inv e0.
+        simpl_tape in IHp. specialize IHp with (2 := Hx) (3 := Hs1) (4 := Hs2) (5 := eq_refl) (6 := eq_refl). spec_assert IHp by auto.
+        simpl_list; cbn; auto.
+    - exfalso. destruct str1 as [ | s str1]; cbn in *.
+      + apply midtape_tape_local_cons in HT1. apply midtape_tape_local_cons in HT2. rewrite HT1, HT2 in *. cbn in *. inv e; inv e0. rewrite Hx in e2. cbn in e2. congruence.
+      + apply midtape_tape_local_cons in HT1. apply midtape_tape_local_cons in HT2. rewrite HT1, HT2 in *. cbn in *. inv e; inv e0.
+        specialize (Hstr1 c2 ltac:(auto)). rewrite Hstr1 in e1. cbn in e1. congruence.
+    - exfalso. destruct str1 as [ | s str1]; cbn in *.
+      + apply midtape_tape_local_cons in HT1. apply midtape_tape_local_cons in HT2. rewrite HT1, HT2 in *. cbn in *. auto.
+      + apply midtape_tape_local_cons in HT1. apply midtape_tape_local_cons in HT2. rewrite HT1, HT2 in *. cbn in *. auto.
+  Qed.
+
+
+  Lemma Compare_correct_short_midtape (str1 str2 : list X) (x s1 s2 : X) ls1 rs1 ls2 m rs2 :
+    (forall x, In x str1 -> stop x = false) ->
+    stop m = false ->
+    stop x = false ->
+    stop s1 = true ->
+    stop s2 = true ->
+    Compare_fun stop (midtape ls1 m (str1 ++ x :: str2 ++ s1 :: rs1),
+                      midtape ls2 m (str1 ++ s2 :: rs2)) =
+    (false, (midtape (rev str1 ++ m :: ls1) x (str2 ++ s1 :: rs1),
+             midtape (rev str1 ++ m :: ls2) s2 rs2)).
+  Proof.
+    intros Hstr1 Hm Hx Hs1 Hs2.
+    erewrite Compare_correct_short with (str1 := m :: str1) (str2 := str2) (s1 := s1) (s2 := s2); cbn; eauto.
+    - now simpl_list; cbn.
+    - intros ? [ <- | H]; auto.
+  Qed.
+
+
+  Lemma Compare_correct_long_midtape (str1 str2 : list X) (x s1 s2 : X) ls1 rs1 ls2 m rs2 :
+    (forall x, In x str1 -> stop x = false) ->
+    stop m = false ->
+    stop x = false ->
+    stop s1 = true ->
+    stop s2 = true ->
+    Compare_fun stop (midtape ls2 m (str1 ++ s2 :: rs2),
+                      midtape ls1 m (str1 ++ x :: str2 ++ s1 :: rs1)) =
+    (false, (midtape (rev str1 ++ m :: ls2) s2 rs2,
+             midtape (rev str1 ++ m :: ls1) x (str2 ++ s1 :: rs1))).
+  Proof.
+    change ((midtape ls2 m (str1 ++ s2 :: rs2), midtape ls1 m (str1 ++ x :: str2 ++ s1 :: rs1))) with (swap (midtape ls1 m (str1 ++ x :: str2 ++ s1 :: rs1), midtape ls2 m (str1 ++ s2 :: rs2))).
+    change (midtape (rev str1 ++ m :: ls2) s2 rs2, midtape (rev str1 ++ m :: ls1) x (str2 ++ s1 :: rs1)) with (swap (midtape (rev str1 ++ m :: ls1) x (str2 ++ s1 :: rs1), midtape (rev str1 ++ m :: ls2) s2 rs2)).
+    intros. rewrite Compare_correct_swap. cbn. rewrite Compare_correct_short_midtape; eauto.
+  Qed.
+
+
+  (** Worst-case time (read the full string) *)
+  Lemma Compare_steps_correct (str1 str2 : list X) (s1 s2 : X) rs1 rs2 t :
+    stop s1 = true ->
+    stop s2 = true ->
+    tape_local (fst t) = str1 ++ s1 :: rs1 ->
+    tape_local (snd t) = str2 ++ s2 :: rs2 ->
+    Compare_steps stop t <= 5 + 6 * max (length str1) (length str2).
+  Proof.
+    revert rs1 rs2 str1 str2. functional induction (Compare_steps stop t); intros rs1 rs2 str1 str2; intros Hs1 Hs2 HT1 HT2; destruct t as [t1 t2]; cbn in *.
+    all: try lia. (* this solves all but the inductive case *)
+    destruct str1 as [ | s str1], str2 as [ | s' str2]; cbn in *;
+      apply midtape_tape_local_cons in HT1; apply midtape_tape_local_cons in HT2; rewrite HT1, HT2 in *; cbn in *;
+        inv e; inv e0.
+    - exfalso. rewrite Hs1 in e1. cbn in e1. congruence.
+    - exfalso. rewrite Hs1 in e1. cbn in e1. congruence.
+    - exfalso. rewrite Hs2 in e2. cbn in e2. congruence.
+    - simpl_tape in IHn. specialize IHn with (1 := Hs1) (2 := Hs2) (3 := eq_refl) (4 := eq_refl). lia.
+  Qed.
+
+  Lemma Compare_steps_correct_midtape (str1 str2 : list X) (s1 s2 : X) (m : X) ls1 ls2 rs1 rs2 :
+    stop s1 = true ->
+    stop s2 = true ->
+    Compare_steps stop (midtape ls1 m (str1 ++ s1 :: rs1), midtape ls2 m (str2 ++ s2 :: rs2)) <= 11 + 6 * max (length str1) (length str2).
+  Proof.
+    intros Hs1 Hs2. rewrite Compare_steps_correct with (str1 := m :: str1) (str2 := m :: str2) (s1 := s1) (s2 := s2); cbn; eauto. lia.
+  Qed.
+
+  (* Worst case steps for moving back after comparing *)
+  Lemma Compare_Move_steps_midtape1 (stop' : X -> bool) (str1 str2 : list X) (s1 s2 : X) (m : X) ls1 ls2 rs1 rs2 :
+    (forall x, In x str1 -> stop x = false) ->
+    (forall x, In x str2 -> stop x = false) ->
+    stop m = false ->
+    stop s1 = true ->
+    stop s2 = true ->
+    stop' m = true ->
+    (forall x, In x str1 -> stop' x = false) ->
+    (forall x, In x str2 -> stop' x = false) ->
+    MoveToSymbol_L_steps stop' id (fst (snd (Compare_fun stop (midtape ls1 m (str1 ++ s1 :: rs1), midtape ls2 m (str2 ++ s2 :: rs2))))) <=
+    8 + 4 * length str1.
+  Proof.
+    intros.
+    pose proof compare_lists str1 str2 as[ HC | [ (a&b&l1&l2&l3&HC1&HC2&HC3) | [ (a&l1&l2&HC1&HC2) | (a&l1&l2&HC1&HC2) ]]]; subst.
+    - rewrite Compare_correct_eq_midtape; cbn; auto. rewrite MoveToSymbol_L_steps_midtape; auto. simpl_list. lia.
+    - simpl_list; cbn. rewrite Compare_correct_neq_midtape; cbn; auto. rewrite MoveToSymbol_L_steps_midtape; auto. simpl_list. lia.
+    - simpl_list; cbn. rewrite Compare_correct_short_midtape; cbn; auto. rewrite MoveToSymbol_L_steps_midtape; auto. simpl_list. lia.
+    - simpl_list; cbn. rewrite Compare_correct_long_midtape; cbn; auto. rewrite MoveToSymbol_L_steps_midtape; auto. simpl_list. lia.
+  Qed.
+
+  Lemma Compare_Move_steps_midtape2 (stop' : X -> bool) (str1 str2 : list X) (s1 s2 : X) (m : X) ls1 ls2 rs1 rs2 :
+    (forall x, In x str1 -> stop x = false) ->
+    (forall x, In x str2 -> stop x = false) ->
+    stop m = false ->
+    stop s1 = true ->
+    stop s2 = true ->
+    stop' m = true ->
+    (forall x, In x str1 -> stop' x = false) ->
+    (forall x, In x str2 -> stop' x = false) ->
+    MoveToSymbol_L_steps stop' id (snd (snd (Compare_fun stop (midtape ls1 m (str1 ++ s1 :: rs1), midtape ls2 m (str2 ++ s2 :: rs2))))) <=
+    8 + 4 * length str2.
+  Proof.
+    intros.
+    pose proof compare_lists str1 str2 as[ HC | [ (a&b&l1&l2&l3&HC1&HC2&HC3) | [ (a&l1&l2&HC1&HC2) | (a&l1&l2&HC1&HC2) ]]]; subst.
+    - rewrite Compare_correct_eq_midtape; cbn; auto. rewrite MoveToSymbol_L_steps_midtape; auto. simpl_list. lia.
+    - simpl_list; cbn. rewrite Compare_correct_neq_midtape; cbn; auto. rewrite MoveToSymbol_L_steps_midtape; auto. simpl_list. lia.
+    - simpl_list; cbn. rewrite Compare_correct_short_midtape; cbn; auto. rewrite MoveToSymbol_L_steps_midtape; auto. simpl_list. lia.
+    - simpl_list; cbn. rewrite Compare_correct_long_midtape; cbn; auto. rewrite MoveToSymbol_L_steps_midtape; auto. simpl_list. lia.
+  Qed.
+
+End Compare_fun_lemmas.
