theories/TM/L/Transcode/Enc_to_Boollist.v
@@ -1,0 +1,272 @@
+From Undecidability.L Require Import LTactics Datatypes.Lists Datatypes.LNat Datatypes.LBool.
+From Undecidability.TM Require TM ProgrammingTools CaseList CaseBool ListTM.
+
+From Undecidability.TM Require Import TM_facts SizeBounds L.Transcode.BoollistEnc.
+
+From Undecidability.L.Complexity  Require Import UpToCNary.
+
+From Undecidability.L.AbstractMachines Require Import FlatPro.Programs.
+     
+Unset Printing Coercions.
+
+From Undecidability.TM.L Require Alphabets.
+
+From Coq Require Import Lia Ring Arith.
+
+From Undecidability Require Import TM.Code.List.Concat_Repeat.
+
+Set Default Proof Using "Type".
+
+Module EncToBoollist.
+  Section M.
+    Import ProgrammingTools Combinators App CaseList CaseBool.
+    Import Alphabets.
+
+
+    Variable (sig : finType).
+    (* Hypothesis (defX: inhabitedC sigX). *)
+
+    (* We use the FinType instance of bool, as it has a Case-machine *)
+    
+    Context `{retr__list : Retract (sigList bool) sig}
+            `{retr__Pro : Retract Alphabets.sigPro sig}.
+
+    Local Instance retr__nat : Retract sigNat sig := ComposeRetract retr__Pro _.
+    Local Instance retr__bool : Retract bool sig := ComposeRetract retr__list (Retract_sigList_X _).
+    
+    (* Check _ : codable sig (list bool). *)
+    (* Check _ : codable sig bool. *)
+
+    (* Tapes: 
+       0: compiled and encoded bs (input)
+       1: result 
+       2: intern (constant for ConcatRepeat [0])
+       3: intern (length of bs for concatReepat [1])
+     *)
+    
+    Definition Rel : pRel sig^+ unit 3 :=
+      ignoreParam
+        (fun tin 'tout =>
+           forall (bs : list bool),
+             tin[@Fin0] ≃ compile (Computable.enc bs)
+             -> isVoid tin[@Fin1]
+             -> isVoid tin[@Fin2]
+             -> tout[@Fin0] ≃ concat (repeat enc_bool_closing (length bs))
+               /\ tout[@Fin1]  ≃ rev bs
+               /\ isVoid tout[@Fin2]).
+
+    (* für step (prepend the bs-dependent symbols) 
+               Tapes: 
+       0: bs (input)
+       1: result 
+       2: head of bs
+       3: intern (length of bs for concatReepat [1])
+     *)
+
+     Compute (fun b => enc_bool_nil).
+     Compute (fun b => (enc_bool_perElem true)).
+     Compute (fun b => (enc_bool_perElem false)).
+     From Undecidability Require Import Cons_constant CaseCom CaseNat CaseList.
+
+     Locate M.
+
+    Definition M__step : pTM sig^+ (option unit) 3 :=
+      CaseList _ ⇑ retr__Pro @ [|Fin0;Fin2|];;Reset _ @ [|Fin2|];;
+      CaseList _ ⇑ retr__Pro @ [|Fin0;Fin2|];;Reset _ @ [|Fin2|];;
+      CaseList _ ⇑ retr__Pro @ [|Fin0;Fin2|];;
+      CaseCom ⇑ ComposeRetract _ _ @ [|Fin2|];;
+      If (CaseNat ⇑ _ @ [|Fin2|])
+        (Return (Reset _ @ [|Fin2|];;
+                 CaseList _ ⇑ retr__Pro @ [|Fin0;Fin2|];;Reset _ @ [|Fin2|];;
+                 CaseList _ ⇑ retr__Pro @ [|Fin0;Fin2|];;Reset _ @ [|Fin2|]
+              ) (Some tt))
+        (Reset _ @ [|Fin2|];;
+         CaseList _ ⇑ retr__Pro @ [|Fin0;Fin2|];;Reset _ @ [|Fin2|];;
+         CaseList _ ⇑ retr__Pro @ [|Fin0;Fin2|];;Reset _ @ [|Fin2|];;
+         CaseList _ ⇑ retr__Pro @ [|Fin0;Fin2|];;
+         CaseCom ⇑ ComposeRetract _ _ @ [|Fin2|];;
+         Switch (CaseNat ⇑ _ @ [|Fin2|])
+          (fun b => Cons_constant.M b ⇑ retr__list @[|Fin1|]);;
+          Reset _ @ [|Fin2|];;
+          CaseList _ ⇑ retr__Pro @ [|Fin0;Fin2|];;Reset _ @ [|Fin2|];;
+          CaseList _ ⇑ retr__Pro @ [|Fin0;Fin2|];;Reset _ @ [|Fin2|];;
+          CaseList _ ⇑ retr__Pro @ [|Fin0;Fin2|];;Reset _ @ [|Fin2|];;
+          Return Nop (None)
+        ).
+
+    Definition Rel__step : pRel sig^+ (option unit) 3 :=
+      (fun tin '(yout,tout) =>
+         forall (bs : list bool) (res : list bool) n,
+          tin[@Fin0] ≃ flat_map enc_bool_perElem bs ++ enc_bool_nil ++ concat (repeat enc_bool_closing n)
+           -> tin[@Fin1] ≃ res
+           -> isVoid tin[@Fin2]
+           -> match bs,yout with
+               [],  Some _ => tout[@Fin0] ≃  concat (repeat enc_bool_closing (n + length bs))
+                             /\ tout[@Fin1] = tin[@Fin1]
+              | (b::bs'),None => tout[@Fin0] ≃ flat_map enc_bool_perElem bs' ++ enc_bool_nil ++ concat (repeat enc_bool_closing n)
+                                 /\ tout[@Fin1] ≃ b::res
+              | _,_ => False
+              end
+             /\ isVoid tout[@Fin2]). 
+
+    Local Ltac autoModPon :=
+    repeat match goal with
+    | H : ((_ |_ _) ∘ _) _ _ |- _ =>
+      let tmid := fresh "tmid_" in
+      let H' := fresh H in
+      destruct H as (tmid&H'&H);cbn in H';(modpon H';[])
+    | H : @eq Tok _ _ |- _ => first [discriminate H]
+    | H : ACom2Com ?x = _ |- _ => (is_var x;destruct x;inversion H);let n := numgoals in guard n <= 1
+    | H : match ?x with _ => _ end |- _ => (destruct x eqn:?;try (exfalso;exact H));[]
+    | H : _ |- _ => modpon H;[]
+    end.
+
+    Arguments rcomp : simpl never.
+
+    Lemma Realise__step : M__step ⊨ Rel__step .
+    Proof. 
+      eapply Realise_monotone.
+      {unfold M__step. TM_Correct_noSwitchAuto. TM_Correct.
+       1-2:now eapply RealiseIn_Realise, CaseCom_Sem. intros. TM_Correct. apply Cons_constant.Realise.
+      } 
+      intros t (y,t') H. cbn.
+      TMSimp autoModPon. autoModPon. rewrite app_assoc,enc_boollist_helper in H3;cbn in H3.
+      TMSimp autoModPon. destruct ymid. all:TMSimp autoModPon.
+      unfold enc_bool_nil,enc_bool_perElem in *.
+      TMSimp autoModPon.
+      destruct H as [H|H];cbn in H;TMSimp autoModPon.  
+      { destruct bs. 2:easy. TMSimp autoModPon. rewrite Nat.add_0_r. easy. }
+      destruct bs. easy.
+       TMSimp autoModPon.
+       destruct ymid;TMSimp autoModPon.
+       hnf in H. 
+       TMSimp autoModPon.
+       destruct ymid0,ymid;try contradiction.
+       all:destruct b;inv H22;[].
+       all:TMSimp autoModPon;[].
+       all:setoid_rewrite <- app_assoc in H33.
+       all:easy. 
+    Qed.
+
+    Definition M__loop : pTM sig^+ unit 3 := While M__step.
+
+    Definition Rel__loop : pRel sig^+ (unit) 3 :=
+      (fun tin '(yout,tout) =>
+      forall (bs : list bool) res n,
+       tin[@Fin0] ≃ flat_map enc_bool_perElem bs ++ enc_bool_nil ++ concat (repeat enc_bool_closing n)
+        -> tin[@Fin1] ≃ res
+        -> isVoid tin[@Fin2]
+        -> tout[@Fin0] ≃ concat (repeat enc_bool_closing n)
+        /\ tout[@Fin1] ≃ rev bs ++ res
+        /\ isVoid tout[@Fin2]).
+
+    Lemma Realise__loop : M__loop ⊨ Rel__loop .
+    Proof.
+      eapply Realise_monotone.
+      {unfold M__loop. TM_Correct_noSwitchAuto. TM_Correct. apply Realise__step. }
+      eapply WhileInduction;intros;hnf;intros bs res n Hbs Hres Ht2.
+      -specialize (HLastStep bs). modpon HLastStep;[].
+       destruct bs. 2:easy. TMSimp. rewrite plus_0_r in H. easy.
+      -hnf in HStar. modpon HStar. destruct bs. easy. TMSimp.
+      specialize (HLastStep bs).
+       modpon HLastStep. rewrite <- app_assoc;cbn. easy.
+    Qed.
+    
+    (*
+    Import MoreList.
+    Lemma _Terminates__loop :
+      { time : UpToC (fun l => l + 1) &
+               projT1 M__loop ↓ (Ter' time)}.
+    Proof.
+      evar (c1 : nat). evar (c2 : nat).
+      exists_UpToC (fun l => l * c1 + c2). 2:now smpl_upToC_solve.
+      eapply TerminatesIn_monotone.
+      -unfold M__loop. TM_Correct. now apply Realise__step. now apply Terminates__step.
+      -apply WhileCoInduction. unfold Ter'.
+       intros tin k (bs&res&Hbs&Hres&Hxtin2&Hk).
+       eexists. split.
+       { exists bs,res. repeat simple apply conj. 1-3:eassumption. rewrite UpToC_le. reflexivity. }
+       unfold Rel__step. intros ymid tmid Hstep. modpon Hstep.
+       destruct ymid as [[]| ],bs. all:try now exfalso;eassumption.
+       +cbn [length]. rewrite <- Hk, Nat.mul_0_l, Nat.mul_1_r,!Nat.add_0_l. unfold c2. reflexivity.
+       +TMSimp.
+        eexists. split.
+        *repeat simple eapply ex_intro. repeat simple apply conj. 1-2:now contains_ext. now isVoid_mono. reflexivity.
+        *rewrite <- Hk. ring_simplify. set (c' := c__leUpToC).
+         replace c1 with (c'+1). 2:now unfold c',c1. nia.
+    Qed.
+
+    Definition Terminates__loop := projT2 _Terminates__loop.
+*)
+    Import ListTM.
+    
+    Definition M : pTM sig^+ unit 3 :=
+      WriteValue (encode ([]:list bool)) ⇑ _ @ [|Fin1|];;
+      M__loop.
+
+    Lemma Realise : M ⊨ M.Rel.
+    Proof.
+      eapply Realise_monotone.
+      {unfold M. TM_Correct_noSwitchAuto. TM_Correct. apply Realise__loop. }
+      intros tin (yout,tout) (?&?&?&H). hnf. intros bs Htin1 Htin2 Htin3. hnf in H.
+      rewrite enc_bool_explicit in Htin1.
+      TMSimp autoModPon. specialize (H0 []). TMSimp autoModPon.
+      rewrite app_nil_r in H1. easy.
+    Qed.
+
+    (*
+    Definition Ter time: tRel sig^+ 4 :=
+      (fun tin k =>
+         exists (bs : list bool),
+           tin[@Fin0] ≃ bs 
+           /\ isVoid tin[@Fin1]
+           /\ isVoid tin[@Fin2]
+           /\ isVoid tin[@Fin3]
+           /\ time (length bs) <= k ).
+
+    Lemma _Terminates :
+      { time : UpToC (fun l => l + 1) &
+               projT1 M ↓ Ter time}.
+    Proof.
+      eexists_UpToC time.
+      eapply TerminatesIn_monotone.
+      { unfold M. TM_Correct.
+        all: eauto 2 using App'_Terminates,App'_Realise,Length_Computes,ConcatRepeat.Realise,ConcatRepeat.Terminates,Length_Terminates,Realise__loop.
+        simple apply Terminates__loop. }
+      intros tin k H. hnf in H. destruct H as (bs&Hbs&Hres&Htin2&Htin3&Hl).
+      cbn -[plus]. infTer 3.
+      {
+        unfold Length_T. cbn. eexists. repeat simple apply conj. now contains_ext. 1-3:now isVoid_mono.        
+        rewrite (correct__leUpToC (Length_steps_nice _) bs),(correct__leUpToC boollist_size).  reflexivity.
+      }
+      2:{ intros tout _ (H&Hrem). TMSimp. modpon H.
+          infTer 5. intros t1_ _ (Ht1&Ht1Rem). TMSimp. specialize (Ht1 []). modpon Ht1;[].
+          infTer 5. intros t2_ _ (Ht2&Ht2Rem). TMSimp. modpon Ht2;[].
+          unfold ConcatRepeat.Ter. cbn. 
+          infTer 5. 1:{ repeat simple apply conj. 1,2,3:now contains_ext.  rewrite UpToC_le. reflexivity. }
+          intros t3_ _ (Ht3&Ht3Rem). TMSimp. modpon Ht3;[]. rewrite app_nil_r in Ht4.
+          infTer 4. 1-2:easy. 
+          intros t4 _ (Htp4&Ht4Rem). TMSimp. modpon Htp4;[].
+          infTer 5. intros t5 _ (Htp5&Ht5Rem). TMSimp. modpon Htp5;[].
+          infTer 5.
+          1:{
+            unfold App'_T. cbn. eexists _,_.  repeat simple apply conj. 1,2:simpl_surject;now contains_ext.
+            rewrite (correct__leUpToC (App'_steps_nice _)). reflexivity.
+          }
+          intros t6_ _ Ht6. modpon Ht6;[]. TMSimp.
+          infTer 4. now contains_ext.
+          { unfold Reset_steps. reflexivity. }
+          intros t7 _ Htp7. modpon Htp7;[]. hnf. TMSimp.
+          do 2 eexists. repeat simple apply conj. 1,2:now contains_ext. now isVoid_mono.
+          rewrite UpToC_le. reflexivity.
+      }
+      - rewrite <- Hl.  set (l:=length bs). [time]:intros l.  unfold time. reflexivity.
+      -unfold time. solve [smpl_upToC_solve].
+    Qed.
+
+    Definition Terminates := projT2 _Terminates.
+*)
+  End M.
+End EncToBoollist.
+Arguments EncToBoollist.M : clear implicits.
+Arguments EncToBoollist.M {_} _ _.
